Change update_bytes to call bf_update_range
Looping will be in BFileRec (over chunks) rather than over bytes (as in
SlowByteFile).

src/FastByteFile.v
@@ -94,31 +94,10 @@ Module FASTBYTEFILE.
   Definition hidden (P : Prop) : Prop := P.
   Opaque hidden.
 
-  Definition update_bytes T fsxp inum (off : nat) (newdata : list byte) mscs rx : prog T :=
-    let^ (mscs, finaloff) <- ForEach b rest newdata
-      Ghost [ mbase F Fm A f allbytes ]
-      Loopvar [ mscs boff ]
-      Continuation lrx
-      Invariant
-        exists m' flist' f' allbytes',
-          LOG.rep fsxp.(FSXPLog) F (ActiveTxn mbase m') mscs  *
-          [[ (Fm * BFILE.rep fsxp.(FSXPBlockAlloc) fsxp.(FSXPInode) flist')%pred (list2mem m') ]] *
-          [[ (A * #inum |-> f')%pred (list2nmem flist') ]] *
-          [[ bytes_rep f' allbytes' ]] *
-          [[ apply_bytes allbytes' boff rest = apply_bytes allbytes off newdata ]] *
-          [[ boff <= length allbytes' ]] *
-          [[ off + length newdata = boff + length rest ]] *
-          [[ hidden (length allbytes = length allbytes') ]] *
-          [[ hidden (BFILE.BFAttr f = BFILE.BFAttr f') ]]
-      OnCrash
-        exists m',
-          LOG.rep fsxp.(FSXPLog) F (ActiveTxn mbase m') mscs
-      Begin
-         mscs <- BFileRec.bf_put byte_type items_per_valu itemsz_ok
-            fsxp.(FSXPLog) fsxp.(FSXPInode) inum ($ boff) b mscs;
-          lrx ^(mscs, boff + 1)
-      Rof ^(mscs, off);
-      rx mscs.
+  Definition update_bytes T fsxp inum (off : nat) len (newbytes : bytes len) mscs rx : prog T :=
+    let^ (mscs) <- BFileRec.bf_update_range items_per_valu itemsz_ok
+      fsxp inum off newbytes mscs;
+    rx ^(mscs).
 
   Definition read_byte T fsxp inum (off:nat) mscs rx : prog T :=
   let^ (mscs, b) <- BFileRec.bf_get byte_type items_per_valu itemsz_ok
@@ -349,16 +328,17 @@ Module FASTBYTEFILE.
   Qed.
 
 
-  Theorem update_bytes_ok: forall fsxp inum off newdata mscs,
-      {< m mbase F Fm A flist f bytes olddata Fx,
+  Theorem update_bytes_ok: forall fsxp inum off len (newbytes : bytes len) mscs,
+      {< m mbase F Fm A flist f bytes olddata newdata Fx,
        PRE LOG.rep (FSXPLog fsxp) F (ActiveTxn mbase m) mscs *
            [[ (Fm * BFILE.rep (FSXPBlockAlloc fsxp) (FSXPInode fsxp) flist)%pred (list2mem m) ]] *
            [[ (A * #inum |-> f)%pred (list2nmem flist) ]] *
            [[ rep bytes f ]] *
            [[ (Fx * arrayN off olddata)%pred (list2nmem bytes) ]] *
+           [[ newdata = bsplit_list newbytes ]] *
            [[ hidden (length olddata = length newdata) ]] *
            [[ off + length newdata <= length bytes ]]
-      POST RET:mscs
+      POST RET: ^(mscs)
            exists m', LOG.rep (FSXPLog fsxp) F (ActiveTxn mbase m') mscs *
            exists flist' f' bytes',
            [[ (Fm * BFILE.rep (FSXPBlockAlloc fsxp) (FSXPInode fsxp) flist')%pred (list2mem m') ]] *
@@ -367,68 +347,11 @@ Module FASTBYTEFILE.
            [[ (Fx * arrayN off newdata)%pred (list2nmem bytes') ]] *
            [[ hidden (BFILE.BFAttr f = BFILE.BFAttr f') ]]
        CRASH LOG.would_recover_old (FSXPLog fsxp) F mbase
-      >} update_bytes fsxp inum off newdata mscs.
+      >} update_bytes fsxp inum off newbytes mscs.
   Proof.
     unfold update_bytes, rep, bytes_rep.
-
-    step.   (* step into loop *)
-
-    rewrite firstn_length in *.
-
-    eapply le_trans. eapply le_plus_l. eapply le_trans. apply H4.
-
-    apply Min.le_min_r.
-
-    constructor.
-
-    step.   (* bf_put *)
-
-    erewrite wordToNat_natToWord_bound by eauto.
-    eauto.
-
-    constructor.
-
-
-    step.
-    rewrite length_upd. auto.
-    rewrite <- H21.
-    rewrite <- apply_bytes_upd_comm by omega.
-    unfold upd.
-
-    erewrite wordToNat_natToWord_bound by eauto.
-    auto.
-
-    rewrite length_upd.
-    eauto.
-
-    rewrite H18. rewrite length_upd. constructor.
-    subst; simpl; auto.
-
-    step.
-
-    eexists.
-    intuition.
-    eauto.
-    eauto.
-    rewrite <- H15.
-    rewrite firstn_length in *.
-    rewrite <- H16.
-    eauto.
-
-    rewrite <- H15.
-    rewrite <- H16.
-    eauto.
-
-    rewrite <- H15.
-    eapply apply_bytes_arrayN. eauto.
-    instantiate (olddata := olddata).
-    eauto.
-    eauto.
-
-    apply LOG.activetxn_would_recover_old.
-    Grab Existential Variables.
-    exact tt.
-  Qed.
+    (* XXX: step fails here for some reason *)
+  Admitted.
 
   Hint Extern 1 ({{_}} progseq (update_bytes _ _ _ _ _) _) => apply update_bytes_ok : prog.
 
